\documentclass[8pt,a4paper,landscape]{article}
\usepackage[a4paper,margin=1in,landscape]{geometry}
\usepackage[utf8]{inputenc}
\usepackage{amsmath}
\usepackage{amsfonts}
\usepackage{amssymb}
\usepackage{color}
\usepackage{bussproofs}
\begin{document}
\begin{flalign*}
&Mcons_\alpha       &&: M\alpha &&&&& \\
&Mcons^{st}_\alpha  &&: (\sigma\rightarrow\alpha\sigma) &&&&& \\
&Mcons^{res}_\alpha &&: (\alpha | \epsilon) &&&&&\\
&Mcons^{prs}_\alpha &&: (\sigma \rightarrow ( \sigma \rightarrow(\alpha | \epsilon)\times\sigma)\times\sigma) &&&&& \\
\end{flalign*}

$try^{prs}\:k\:err\:pm = lift^{st}(lift^{st}(try^{res} k (\lambda e_1 . try^{res} (>>=)^{id} (\lambda e_2. fail^{prs}(e_1 + e_2)))err))pm : (\alpha \rightarrow M \beta)\rightarrow
           (\epsilon \rightarrow M \beta)\rightarrow
       Mcons^{prs}_\alpha \rightarrow
       Mcons^{prs}_\beta $ \\

\begin{prooftree}
  \AxiomC{$try^{res}$ $:
           (\alpha \rightarrow M \beta)\rightarrow
           (\epsilon \rightarrow M \beta)\rightarrow
           Mcons^{res}_\alpha\rightarrow
           Mcons^{res}_\beta$}
  \AxiomC{$(>>=)^{id} : (\alpha \rightarrow M \beta)$}
\BinaryInfC{$try^{res} (>>=)^{id} :
            (\epsilon \rightarrow M \beta)\rightarrow
            Mcons^{res}_\alpha\rightarrow
            Mcons^{res}_\beta$}
    \AxiomC{$fail^{prs} :
             \epsilon \rightarrow Mcons^{prs}_\alpha $}
      \AxiomC{$e_1 : \epsilon$}
      \AxiomC{$e_2 : \epsilon$}
    \BinaryInfC{$e_1+e_2 :\epsilon$}
  \BinaryInfC{$fail^{prs} (e_1+e_2) :
               Mcons^{prs}_\alpha$}
  \UnaryInfC{$\lambda e_2 . fail^{prs} (e_1+e_2) :
              \epsilon \rightarrow Mcons^{prs}_\alpha$}
\BinaryInfC{$try^{res} (>>=)^{id}\:(\lambda e_2. fail^{prs}(e_1 + e_2)) :
             Mcons^{res}_\alpha\rightarrow Mcons^{res}_\beta$}
\UnaryInfC{$\lambda e_1 . try^{res} (>>=)^{id}\:(\lambda e_2. fail^{prs}(e_1 + e_2)) :
            \epsilon \rightarrow Mcons^{res}_\alpha\rightarrow Mcons^{res}_\beta$}
\end{prooftree}

\begin{prooftree}
  \AxiomC{$try^{res} :
           (\alpha \rightarrow M \beta)\rightarrow
               (\epsilon \rightarrow M \beta)\rightarrow
           Mcons^{res}_\alpha\rightarrow
           Mcons^{res}_\beta$}
  \AxiomC{$k:(\alpha\rightarrow M \beta)$}
\BinaryInfC{$try^{res}k :
                 $\textcolor{red}{$(\epsilon \rightarrow M \beta)$} $\rightarrow
         Mcons^{res}_\alpha\rightarrow
         Mcons^{res}_\beta$}
\AxiomC{$\lambda e_1 . try^{res} (>>=)^{id}\:(\lambda e_2. fail^{prs}(e_1 + e_2)) :
         $\textcolor{red}{$\epsilon \rightarrow Mcons^{res}_\alpha\rightarrow Mcons^{res}_\beta$}}
\BinaryInfC{\textbf{Contradiction:} application of $try^{res}\:k$ expects $(\epsilon \rightarrow M \beta)$ but got $(\epsilon \rightarrow Mcons^{res}_\alpha\rightarrow Mcons^{res}_\beta)$}
\end{prooftree}

\newpage

$try^{prs}\:k\:err\:pm = lift^{st}(lift^{st\_ctxt}(try^{res} k (\lambda e_1 . try^{res} return^{id} (\lambda e_2. fail^{prs}(e_1 + e_2)))err))pm : (\alpha \rightarrow  Mcons^{prs}_\beta)\rightarrow
           (\epsilon \rightarrow Mcons^{prs}_\beta)\rightarrow
       Mcons^{prs}_\alpha \rightarrow
       Mcons^{prs}_\beta $ \\

\begin{prooftree}
  \AxiomC{$try^{res}$ $:
           (\alpha \rightarrow Mcons^{res}_\beta)\rightarrow
           (\epsilon \rightarrow Mcons^{res}_\beta)\rightarrow
           Mcons^{res}_\alpha\rightarrow
           Mcons^{res}_\beta$}
  \AxiomC{$return^{id} : (\alpha \rightarrow Mcons^{res}_\beta)$}
\BinaryInfC{$try^{res} return^{id} :
            (\epsilon \rightarrow Mcons^{res}_\beta)\rightarrow
            Mcons^{res}_\alpha\rightarrow
            Mcons^{res}_\beta$}
    \AxiomC{$fail^{prs} :
             \epsilon \rightarrow Mcons^{prs}_\alpha $}
      \AxiomC{$e_1 : \epsilon$}
      \AxiomC{$e_2 : \epsilon$}
    \BinaryInfC{$e_1+e_2 :\epsilon$}
  \BinaryInfC{$fail^{prs} (e_1+e_2) :
               Mcons^{prs}_\alpha$}
  \UnaryInfC{$\lambda e_2 . fail^{prs} (e_1+e_2) :
              \epsilon \rightarrow Mcons^{prs}_\alpha$}
\BinaryInfC{$try^{res} return^{id}\:(\lambda e_2. fail^{prs}(e_1 + e_2)) :
             Mcons^{res}_\alpha\rightarrow Mcons^{res}_\beta$}
\AxiomC{$err : Mcons^{res}_\alpha$}
\BinaryInfC{$try^{res} return^{id}\:(\lambda e_2. fail^{prs}(e_1 + e_2)) err :
             Mcons^{res}_\beta$}
\UnaryInfC{$\lambda e_1 . try^{res} return^{id}\:(\lambda e_2. fail^{prs}(e_1 + e_2))err :
            \epsilon \rightarrow Mcons^{res}_\beta$}
\end{prooftree}

\begin{prooftree}
  \AxiomC{$try^{res} :
           (\alpha \rightarrow Mcons^{res}_\beta)\rightarrow
               (\epsilon \rightarrow Mcons^{res}_\beta)\rightarrow
           Mcons^{res}_\alpha\rightarrow
           Mcons^{res}_\beta$}
  \AxiomC{$k:(\alpha\rightarrow Mcons^{prs}_\beta)$}
\BinaryInfC{$try^{res}k :
                 (\epsilon \rightarrow Mcons^{res}_\beta)\rightarrow
         Mcons^{res}_\alpha\rightarrow
         Mcons^{res}_\beta$}
\AxiomC{$\lambda e_1 . try^{res} return^{id}\:(\lambda e_2. fail^{prs}(e_1 + e_2))err :
            \epsilon \rightarrow Mcons^{res}_\beta$}
\BinaryInfC{$try^{res}k\:(\lambda e_1 . try^{res} return^{id}\:(\lambda e_2. fail^{prs}(e_1 + e_2))err) :
            Mcons^{res}_\alpha\rightarrow
         Mcons^{res}_\beta$ }
\end{prooftree}

\begin{prooftree}
\AxiomC{$lift^{st}:(\alpha \rightarrow \beta) \rightarrow Mcons^{st}_\alpha \rightarrow Mcons^{st}_\beta$}
\AxiomC{$lift^{st}:(\alpha \rightarrow \beta) \rightarrow Mcons^{st}_\alpha \rightarrow Mcons^{st}_\beta$}
\AxiomC{$try^{res}k\:(\lambda e_1 . try^{res} return^{id}\:(\lambda e_2. fail^{prs}(e_1 + e_2))\:err) :
         Mcons^{res}_\beta$}
\BinaryInfC{$lift^{st\_ctxt}(try^{res}k\:(\lambda e_1 . try^{res} return^{id}\:(\lambda e_2. fail^{prs}(e_1 + e_2))\:err)\:pm) :
         Mcons^{res}_\beta$ }
\BinaryInfC{$lift^{st}(lift^{st\_ctxt}(try^{res}k\:(\lambda e_1 . try^{res} return^{id}\:(\lambda e_2. fail^{prs}(e_1 + e_2))\:err)\:pm)) :
         Mcons^{res}_\beta$ }
\end{prooftree}

\end{document}
